\documentclass[a4paper]{article}
\usepackage{tasks}
\usepackage{amsmath}
\begin{document}
     \begin{itemize}
  \begin{section}{Polynomials}
  \begin{itemize}
    \item Dividide these polinomials using Ruffini's rule
    \begin{tasks}(2)
      \task $\left(-2 x^{4} -2 x^{3} -9 x^{2} -4 x + 4 \right) : \left( x -7 \right)$
      \task $\left(4 x^{3} -5 x^{2}  + 3 \right) : \left( x + 3 \right)$
      \task $\left(6 x^{2} -7 x -6 \right) : \left( x + 8 \right)$
      \task $\left(-6 x^{2} + 2 x -2 \right) : \left( x -2 \right)$
    \end{tasks}
    \item Dividide these polinomials
    \begin{tasks}(2)
      \task $\left(20 x^{3} + 8 x^{2} -22 x + 4 \right) : \left(-4 x^{2} -4 x + 2 \right)$
      \task $\left(9 x^{3} -3 x^{2} -27 x -10 \right) : \left(-3 x^{2} + 4 x + 5 \right)$
      \task $\left(3 x^{3} + 2 x^{2} -6 x + 1 \right) : \left( x^{2}  -2 \right)$
      \task $\left(-6 x^{3} + 11 x^{2} -1 x + 1 \right) : \left(-2 x^{2} +  x + 1 \right)$
    \end{tasks}
    \item Expand these algebraic identities
    \begin{tasks}(2)
      \task $\left(t - 4 m\right)^2 = {}$
      \task $\left(x + 5 z\right) \cdot \left(x - 5 z\right) = {}$
      \task $\left(5 z^{4} + y^{4}\right) \cdot \left(5 z^{4} - y^{4}\right) = {}$
      \task $\left(5 t^{4} - 3 x^{4}\right)^2 = {}$
      \task $\left(\frac{13}{5} y^{4} - 4 z^{4}\right)^2 = {}$
      \task $\left(\frac{9}{5} m^{3} - 4 y^{3}\right)^2 = {}$
    \end{tasks}
    \item Write these polynomials as an algebraic identity
    \begin{tasks}(2)
      \task $z^{2} -10 x z +25 x^{2} = {}$
      \task $z^{2} -2 b z +b^{2} = {}$
      \task $x^{6} -6 x^{3} y^{3} +9 y^{6} = {}$
      \task $\frac{121}{9} z^{8} -\frac{44}{3} x^{4} z^{4} +4 x^{8} = {}$
    \end{tasks}
    \item Extract common factor from these polynomials
    \begin{tasks}(2)
      \task $-2 x^{3} z^{2} +8 x^{2} z^{2} -8 x z^{2} = {}$
      \task $12 a^{5} x^{7} +20 a^{5} x^{6} -12 a^{5} x^{5} = {}$
      \task $-2 x^{4} y^{4} -10 x^{4} y^{3} +2 x^{4} y^{2} = {}$
    \end{tasks}
  \end{itemize}
  \end{section}
  \begin{section}{Answers}
    \begin{tasks}(2)
      \task $Q(x)=-2 x^{3} -16 x^{2} -121 x -851 $; $R=-5953 $ 
      \task $Q(x)=4 x^{2} -17 x + 51 $; $R=-150 $ 
      \task $Q(x)=6 x -55 $; $R=434 $ 
      \task $Q(x)=-6 x -10 $; $R=-22 $ 
    \end{tasks}
    \begin{tasks}(2)
      \task $Q(x)=-5 x + 3 $; $R=-2 $ 
      \task $Q(x)=-3 x -3 $; $R=5 $ 
      \task $Q(x)=3 x + 2 $; $R=5 $ 
      \task $Q(x)=3 x -4 $; $R=5 $ 
    \end{tasks}
    \begin{tasks}(2)
      \task $t^{2} -8 m t +16 m^{2}$ 
      \task $x^{2} -25 z^{2}$ 
      \task $25 z^{8} -y^{8}$ 
      \task $25 t^{8} -30 t^{4} x^{4} +9 x^{8}$ 
      \task $\frac{169}{25} y^{8} -\frac{104}{5} y^{4} z^{4} +16 z^{8}$ 
      \task $\frac{81}{25} m^{6} -\frac{72}{5} m^{3} y^{3} +16 y^{6}$ 
    \end{tasks}
    \begin{tasks}(2)
      \task $\left(z - 5 x\right)^2$ 
      \task $\left(z - b\right)^2$ 
      \task $\left(x^{3} - 3 y^{3}\right)^2$ 
      \task $\left(\frac{11}{3} z^{4} - 2 x^{4}\right)^2$ 
    \end{tasks}
    \begin{tasks}(2)
      \task $2 x z^{2} \cdot \left(-x^{2} +4 x -4\right)$ 
      \task $4 a^{5} x^{5} \cdot \left(3 x^{2} +5 x -3\right)$ 
      \task $2 x^{4} y^{2} \cdot \left(-y^{2} -5 y +1\right)$ 
    \end{tasks}
  \end{section}
     \end{itemize}
\end{document}